Update translation of inferencer

compiler/bootstrap/translation/compilerMLScript.sml
@@ -2,22 +2,37 @@ open HolKernel Parse boolLib bossLib;
 open preamble;
 open cmlParseTheory cmlPEGTheory;
 open inferTheory
+open terminationTheory
 open ml_translatorLib ml_translatorTheory;
 
 val _ = new_theory "compilerML"
 
 val _ = std_preludeLib.std_prelude ();
 
+val RW = REWRITE_RULE
+val RW1 = ONCE_REWRITE_RULE
+fun list_dest f tm =
+  let val (x,y) = f tm in list_dest f x @ list_dest f y end
+  handle HOL_ERR _ => [tm];
+val dest_fun_type = dom_rng
+val mk_fun_type = curry op -->;
+fun list_mk_fun_type [ty] = ty
+  | list_mk_fun_type (ty1::tys) =
+      mk_fun_type ty1 (list_mk_fun_type tys)
+  | list_mk_fun_type _ = fail()
+
+(* translator setup *)
+
+val _ = register_type ``:lexer_fun$symbol``;
+
 val _ = add_preferred_thy "-";
+val _ = add_preferred_thy "termination";
 
 val NOT_NIL_AND_LEMMA = prove(
   ``(b <> [] /\ x) = if b = [] then F else x``,
   Cases_on `b` THEN FULL_SIMP_TAC std_ss []);
 
 val extra_preprocessing = ref [MEMBER_INTRO,MAP];
-
-val RW = REWRITE_RULE
-val RW1 = ONCE_REWRITE_RULE
 
 fun def_of_const tm = let
   val res = dest_thy_const tm handle HOL_ERR _ =>
@@ -27,7 +42,8 @@ fun def_of_const tm = let
     DB.fetch thy (name ^ "_def") handle HOL_ERR _ =>
     DB.fetch thy (name ^ "_DEF") handle HOL_ERR _ =>
     DB.fetch thy name
-  val def = def_from_thy (#Thy res) name handle HOL_ERR _ =>
+  val def = def_from_thy "termination" name handle HOL_ERR _ =>
+            def_from_thy (#Thy res) name handle HOL_ERR _ =>
             failwith ("Unable to find definition of " ^ name)
   val def = def |> RW (!extra_preprocessing)
                 |> CONV_RULE (DEPTH_CONV BETA_CONV)
@@ -36,8 +52,6 @@ fun def_of_const tm = let
   in def end
 
 val _ = (find_def_for_const := def_of_const);
-
-val _ = register_type ``:lexer_fun$symbol``;
 
 (* parsing: peg_exec and cmlPEG *)
 
@@ -51,9 +65,6 @@ val INTRO_FLOOKUP = prove(
        NONE => Result NONE
      | SOME x => EV x i r y fk)``,
   SRW_TAC [] [finite_mapTheory.FLOOKUP_DEF]);
-
-val RW = REWRITE_RULE
-val RW1 = ONCE_REWRITE_RULE
 
 val _ = translate (def_of_const ``coreloop`` |> RW [INTRO_FLOOKUP]
                    |> SPEC_ALL |> RW1 [FUN_EQ_THM]);
@@ -80,7 +91,6 @@ val _ = (extra_preprocessing :=
 val _ = translate (def_of_const ``ptree_Expr``);
 val _ = translate (def_of_const ``ptree_TopLevelDecs``);
 
-
 (* parsing: top-level parser *)
 
 val _ = translate (RW [monad_unitbind_assert] parse_prog_def);
@@ -96,8 +106,6 @@ val parse_prog_side_def = prove(
   THEN FULL_SIMP_TAC std_ss [INTRO_FLOOKUP] THEN POP_ASSUM MP_TAC
   THEN CONV_TAC (DEPTH_CONV ETA_CONV) THEN FULL_SIMP_TAC std_ss [])
   |> update_precondition;
-
-val _ = ml_translatorLib.print_asts:=true;
 
 (* type inference: t_walkstar and t_unify *)
 
@@ -273,5 +281,193 @@ val ts_unify_side_def = store_thm("ts_unify_side_def",
 val _ = save_thm("anub_ind",REWRITE_RULE[MEMBER_INTRO]miscTheory.anub_ind)
 val _ = translate (REWRITE_RULE[MEMBER_INTRO] miscTheory.anub_def)
 
-(* rest of inferencer TODO*)
+val _ = (extra_preprocessing :=
+  [MEMBER_INTRO, MAP, OPTION_BIND_THM, st_ex_bind_def,
+   st_ex_return_def, failwith_def, guard_def, read_def, write_def]);
+
+val _ = translate (def_of_const``lookup_st_ex``)
+val _ = translate (def_of_const ``fresh_uvar``)
+val _ = translate (def_of_const ``n_fresh_uvar``)
+val _ = translate (def_of_const ``init_infer_state``)
+val _ = translate (def_of_const ``init_state``)
+val _ = translate (def_of_const ``get_next_uvar``)
+val _ = translate (def_of_const ``infer_deBruijn_subst``)
+val _ = translate (def_of_const ``generalise``)
+val _ = translate (def_of_const ``infer_type_subst``)
+
+val _ = translate rich_listTheory.COUNT_LIST_AUX_def
+val _ = translate rich_listTheory.COUNT_LIST_compute
+
+val pair_abs_hack = prove(
+  ``(\(v2:string,v1:infer_t). (v2,0,v1)) =
+    (\v3. case v3 of (v2,v1) => (v2,0:num,v1))``,
+  SIMP_TAC (srw_ss()) [FUN_EQ_THM,FORALL_PROD]);
+
+fun fix_infer_induction_thm def = let
+  val const = def |> SPEC_ALL |> CONJUNCTS |> hd |> SPEC_ALL |> concl
+                  |> dest_eq |> fst |> repeat rator
+  val cname = const |> dest_const |> fst
+  val ind_name = cname ^ "_ind"
+  val ind = fetch "infer" ind_name
+  val s_var = mk_var("state", ``: (num |-> infer_t) infer_st``)
+  val cs = ind |> SPEC_ALL |> UNDISCH_ALL |> CONJUNCTS |> map concl
+               |> map (fn tm => let val xs = list_dest dest_forall tm
+                                    val vs = butlast xs
+                                    val body = repeat rator (last xs)
+                                    in (vs,body) end)
+  fun list_dest_fun_type ty = let
+    val (ty1,ty2) = dest_fun_type ty
+    in ty1 :: list_dest_fun_type ty2 end handle HOL_ERR _ => [ty]
+  fun new_P_inst (vs,P) = let
+    val (Pname,ty) = dest_var P
+    val tys = list_dest_fun_type ty
+    val tys1 = butlast tys @ [type_of s_var, last tys]
+    val Pnew = mk_var(Pname,list_mk_fun_type tys1)
+    val tm = mk_forall(s_var,list_mk_comb(Pnew,vs @ [s_var]))
+    in (Pnew,list_mk_abs(vs,tm)) end
+  val ps = map new_P_inst cs
+  val ind = ind |> SPECL (map snd ps) |> CONV_RULE (DEPTH_CONV BETA_CONV)
+                |> GENL (map fst ps) |> PURE_REWRITE_RULE [pair_abs_hack]
+  val _ = print ("Improved induction theorem: " ^ ind_name ^ "\n")
+  val _ = save_thm(ind_name,ind)
+  in () end handle HOL_ERR _ => ();
+
+val if_apply = prove(
+  ``!b. (if b then x1 else x2) x = if b then x1 x else x2 x``,
+  Cases THEN SRW_TAC [] []);
+
+val option_case_apply = prove(
+  ``!oo. option_CASE oo x1 x2 x = option_CASE oo (x1 x) (\y. x2 y x)``,
+  Cases THEN SRW_TAC [] []);
+
+val pr_CASE = prove(
+  ``pair_CASE (x,y) f = f x y``,
+  SRW_TAC [] []);
+
+val op_apply = prove(
+  ``!op. (ast$op_CASE op x1 x2 x3 x4 x5 x6 x7 x8 x9 x10 x11 x12 x13 x14 x15 x16 x17 x18 x19 x20 x21 x22 x23 x24 x25 x26 x27 x28 x29) y =
+         (ast$op_CASE op
+            (\z. x1 z y)
+            (\z. x2 z y)
+            (\z1 z2. x3 z1 z2 y)
+            (\z1 z2 z3. x4 z1 z2 z3 y)
+            (x5 y) (x6 y) (x7 y) (x8 y) (x9 y) (x10 y) (x11 y) (x12 y) (x13 y)
+            (\z. x14 z y) (\z. x15 z y)
+            (x16 y) (x17 y)
+            (\z. x18 z y)
+            (x19 y) (x20 y) (x21 y) (x22 y) (x23 y) (x24 y) (x25 y) (x26 y) (x27 y) (x28 y)
+            (\z. x29 z y))``,
+  Cases THEN SRW_TAC [] []);
+
+val list_apply = prove(
+  ``!op. (list_CASE op x1 x2) y =
+         (list_CASE op (x1 y) (\z1 z2. x2 z1 z2 y))``,
+  Cases THEN SRW_TAC [] []);
+
+fun full_infer_def aggressive const = let
+  val def = if aggressive then
+              def_of_const const
+              |> RW1 [FUN_EQ_THM]
+              |> RW [op_apply,if_apply,option_case_apply,pr_CASE]
+              |> SIMP_RULE std_ss [op_apply,if_apply,
+                   option_case_apply,list_apply]
+            else
+              def_of_const const
+              |> RW1 [FUN_EQ_THM]
+              |> RW [op_apply,if_apply,option_case_apply]
+              |> CONV_RULE (DEPTH_CONV PairRules.PBETA_CONV)
+  val def = let
+    val s_var = mk_var("state", ``: (num |-> infer_t) infer_st``)
+    val s = def |> SPEC_ALL |> CONJUNCTS |> hd |> SPEC_ALL |> concl
+                |> dest_eq |> fst |> rand |> type_of
+    val def = INST_TYPE (match_type s (type_of s_var)) def
+    in def end handle HOL_ERR _ => def
+  val () = fix_infer_induction_thm def
+  in def end
+
+val infer_def = full_infer_def false;
+val aggr_infer_def = full_infer_def true;
+
+val _ = translate (infer_def ``apply_subst``);
+val _ = translate (infer_def ``apply_subst_list``);
+val _ = translate (infer_def ``add_constraint``);
+val _ = translate (infer_def ``add_constraints``);
+val _ = translate (aggr_infer_def ``constrain_op``);
+val _ = translate (infer_def ``t_to_freevars``);
+
+val _ = translate (typeSystemTheory.build_ctor_tenv_def
+                   |> CONV_RULE(((STRIP_QUANT_CONV o funpow 3 RAND_CONV o
+                                  funpow 2 (LAND_CONV o PairRules.PABS_CONV) o
+                                  funpow 2 RAND_CONV o funpow 2 LAND_CONV)
+                                 (ONCE_REWRITE_CONV [GSYM ETA_AX]))))
+
+val EVERY_INTRO = prove(
+  ``(!x::set s. P x) = EVERY P s``,
+  SIMP_TAC std_ss [res_quanTheory.RES_FORALL,EVERY_MEM]);
+
+val EVERY_EQ_EVERY = prove(
+  ``!xs. EVERY P xs = EVERY I (MAP P xs)``,
+  Induct THEN SRW_TAC [] []);
+
+val _ = translate (infer_def ``check_freevars``
+                   |> RW1 [EVERY_EQ_EVERY])
+
+val _ = translate (infer_def ``check_dup_ctors``
+                   |> SIMP_RULE std_ss [EVERY_INTRO,LET_DEF])
+
+val _ = translate (infer_def ``check_ctor_tenv``)
+
+val _ = translate (infer_def ``is_value``
+            |> RW1 [prove(``~b <=> (b = F)``,SIMP_TAC std_ss [])]
+            |> RW1 [EVERY_EQ_EVERY])
+
+val _ = translate (infer_def ``infer_p``)
+val _ = translate (infer_def ``infer_e``)
+val _ = translate (infer_def ``infer_d``)
+val _ = translate (infer_def ``infer_ds``)
+val _ = translate (infer_def ``check_weakE``)
+val _ = translate (infer_def ``check_specs``)
+val _ = translate (infer_def ``check_signature``)
+val _ = translate (infer_def ``infer_top``)
+
+val infer_prog_def = prove(``
+  (∀idecls ienv x.
+      infer_prog idecls ienv [] x =
+      (Success (empty_inf_decls,(FEMPTY,FEMPTY),FEMPTY,([],[]),[]),x)) ∧
+   ∀idecls ienv top ds x.
+     infer_prog idecls ienv (top::ds) x =
+     case infer_top idecls ienv top x of
+       (Success y,s) =>
+         (case
+            infer_prog (append_decls (FST y) idecls)
+              (ienv with <|inf_t := merge_mod_env (FST (SND y)) ienv.inf_t;
+                inf_c :=
+                  merge_alist_mod_env (FST (SND (SND (SND y))))
+                    ienv.inf_c;
+                inf_v := SND (SND (SND (SND y))) ++ ienv.inf_v;
+                inf_m := FST (SND (SND y)) ⊌ ienv.inf_m|>) ds s
+          of
+            (Success y',s) =>
+              (Success
+                 (append_decls (FST y') (FST y),
+                  merge_mod_env (FST (SND y')) (FST (SND y)),
+                  FST (SND (SND y')) ⊌ FST (SND (SND y)),
+                  merge_alist_mod_env (FST (SND (SND (SND y'))))
+                    (FST (SND (SND (SND y)))),
+                  SND (SND (SND (SND y'))) ++ SND (SND (SND (SND y)))),
+               s)
+          | (Failure e,s) => (Failure e,s))
+     | (Failure e,s) => (Failure e,s)``,
+     rw[infer_prog_def]>>EVAL_TAC>>
+     BasicProvers.EVERY_CASE_TAC>>PairCases_on`a`>>
+     fs[]>>
+     PairCases_on`a'`>>fs[])
+
+(* translating infer ``infer_prog`` doesn't work, maybe because
+  there is an explicit record not written as an update inside
+*)
+val _ = translate infer_prog_def
+
+val _ = translate (infer_def ``infertype_prog``)
+
 val _ = export_theory();
